\chapter{Deriving the steady-state equation}
\label{apndx:derivSS}
\hspace{\parindent} Setting $\frac{d\vec{n}}{dt} = 0$,

\begin{align}
\frac{d}{dt}n_{c} & = 0\\
a(f+f'-f'f)n_{s} - bg'n_{c} & = 0\\
a(f+f'-f'f)n_{s} & = bg'n_{c} \\
\end{align}

Note: $N = n_{c} + n_{s}, n_{s} = N - n{c}$, and $f = 0$.

\begin{equation}
af'(N - n{c}) = bg'n_{c} \\
\label{eq:noFunc}
\end{equation}

Plugging in \eqref{eq:f'} and \eqref{eq:g'} to \eqref{eq:noFunc}:

\begin{align}
a(\alpha\frac{n_{c}}{N-1})(N - n_{c}) &= b(\frac{1}{1 + \frac{\beta n_{c}}{N-1}})(n_{c}) \\
\frac{a\alpha (N - n_{c})}{N-1}n_{c} &= b\frac{N-1}{N-1+\beta n_{c}}n_{c} \\
a\alpha (N - n_{c}) &= b\frac{(N-1)^2}{N-1+\beta n_{c}} \\
a\alpha(N-n_{c})(N-1 + \beta n_{c}) & = b(N-1)^{2}
\end{align}