\chapter{Combined probability of functions $f$ and $f'$}
\label{apndx:prob}

\hspace{\parindent} The forcing function $f$ permits agents to undergo $\mathrm{R_{1}}$ and is represented with a probability $p_{1}$.
The probability that $\mathrm{R_{1}}$ does not occur is $q_{1} = 1 - p_{1}$.
Likewise for the function $f'$ to undergo $\mathrm{R_{1}}$ is represented with a probability $p_{2}$, and non-occurring probability $q_{2}$.
Combining the probabilities $p$ and $q$ results to

\begin{eqnarray}
\label{eqn:conservP1}
p_{1} + q_{1} &&= 1 \\
\label{eqn:conservP2}
p_{2} + q_{2} &&= 1
\end{eqnarray}

Multiplying the equations \eqref{eqn:conservP1} and \eqref{eqn:conservP2} and simplifying

\begin{eqnarray}
(p_{1} + q_{1})(p_{2} + q_{2}) &&= 1 \\
p_{1}p_{2} + p_{1}q_{2} + p_{2}q_{1} + q_{1}q_{2} &&= 1
\end{eqnarray}

$q_{1}q_{2}$ represents neither event occuring thus

\begin{eqnarray}
p_{net} = 1 - q_{1}q_{2} &&= 1 - (1-p_{1})(1-p_{2}) \\
&&= 1 - (1 - p_{1} - p_{2} + p_{1}p_{2}) \\
&&= p_{1} + p_{2} - p_{1}p_{2}
\label{eq:simpleProb}
\end{eqnarray}

Replacing \eqref{eq:simpleProb} with the functions gives
\begin{equation}
p_{net} = f + f' - f'f
\end{equation}
which is used in \eqref{eq:p(r1)}